Added structuring types to RG inductive operations and equivalences on them

project/inductive/basic/inductive_graph_basic_to_RG.v
@@ -55,42 +55,59 @@ Notation "g1 I== g2" := (IG_basic_equiv g1 g2) (at level 80).
 (* Now go to proving that the implementations from IG basic relate to the RG ones *)
 (* Filling in all the admitteds, should suffice to show that IG_basic operations are equivalent to RG operations *)
 (* Hence, all theorems from one apply to the other *)
+Definition IG_basic_Propify_isEmpty (result : bool) : Prop :=
+  match result with
+    | true => True
+    | false => False
+  end
+.
+
+Print NatSet.
+
+(* The "0" is a dummy value, since IG_basic does not return any kind of label *)
+Definition IG_basic_Propify_match (result : option (NatSet.t * NatSet.t) * IG_basic) : (@RG_Decomp nat unit) :=
+  match result with
+    | (Some (froms, tos), rest) => ((True,  (
+                                              fun (label : unit) (other : nat) => NatSet.In other froms,
+                                              0,
+                                              fun (label : unit) (other : nat) => NatSet.In other tos
+                                            ), IG_basic_to_RG_unlE rest))
+    | (None, same)                => ((False, (fun x y => False, 0, fun x y => False)), IG_basic_to_RG_unlE same)
+  end
+.
+
+Definition IG_basic_Propify_labNodes (result : list Node) : Ensemble Node :=
+  cListToEnsemble result.
+
+
+
 (*   {-# MINIMAL empty, isEmpty, match, mkGraph, labNodes #-} *)
-Definition IG_basic_Propify_isEmpty (result : bool) : Prop.
-Proof.
-Admitted.
-
-Definition IG_basic_Propify_match (result : option (NatSet.t * NatSet.t) * IG_basic) : (Prop * Context nat unit) * RG_unlE nat.
-Proof.
-Admitted.
-
-Definition IG_basic_Propify_labNodes (result : list Node) : Ensemble Node.
-Proof.
-Admitted.
-
-
 Theorem IG_basic_empty_relate :
-  IG_basic_to_RG_unlE IG_basic_empty = RG_empty.
+  IG_basic_to_RG_unlE IG_basic_empty === RG_empty.
 Proof.
-Admitted.
+  firstorder.
+Qed.
+
 
 Theorem IG_basic_isEmpty_relate : forall (ig : IG_basic),
-  IG_basic_Propify_isEmpty (IG_basic_isEmpty ig) = RG_isEmpty (IG_basic_to_RG_unlE ig).
+  IG_basic_Propify_isEmpty (IG_basic_isEmpty ig) <-> RG_isEmpty (IG_basic_to_RG_unlE ig).
 Proof.
+  split; intros.
+  - 
 Admitted.
 
 
 Theorem IG_basic_match_relate : forall (node : Node) (ig : IG_basic),
-  IG_basic_Propify_match (IG_basic_match node ig) = RG_match node (IG_basic_to_RG_unlE ig).
+  IG_basic_Propify_match (IG_basic_match node ig) D== RG_match node (IG_basic_to_RG_unlE ig).
 Proof.
 Admitted.
 
 Theorem IG_basic_mkGraph_relate : forall (nodes : list Node) (edges : list (Node * Node)),
-  IG_basic_to_RG_unlE (IG_basic_mkGraph nodes edges) = RG_mkGraph nodes (map (fun '(n1, n2) => (n1, n2, tt)) edges).
+  IG_basic_to_RG_unlE (IG_basic_mkGraph nodes edges) === RG_mkGraph nodes (map (fun '(n1, n2) => (n1, n2, tt)) edges).
 Proof.
 Admitted.
 
 Theorem IG_basic_labNodes_relate : forall (ig : IG_basic),
-  IG_basic_Propify_labNodes (IG_basic_labNodes ig) = RG_labNodes (IG_basic_to_RG_unlE ig).
+  IG_basic_Propify_labNodes (IG_basic_labNodes ig) S== RG_labNodes (IG_basic_to_RG_unlE ig).
 Proof.
 Admitted.
