project/relational_graph_IG_operations.v
@@ -37,13 +37,16 @@ Require Import MyProject.project.util.util.
 
 (* A "set" of adjacencies with the edge label and the label of the neighbour  *)
 (* type Adj b = [(b, Node)] *)
-Definition Adj (A B : Type) := B -> A -> Prop.
+Definition RG_Adj (A B : Type) := B -> A -> Prop.
 
 (* type Context a b  = (Adj b,Node,a,Adj b) *)
-Definition Context (A B : Type) := (Adj A B * A * Adj A B)%type.
+Definition RG_Context (A B : Type) := (RG_Adj A B * A * RG_Adj A B)%type.
+
+(* type Decomp g a b = (MContext a b,g a b) *)
+Definition RG_Decomp (A B : Type) := ((Prop * RG_Context A B) * RG A B)%type.
 
 (* type LEdge b = (Node,Node,b) *)
-Definition Edge (A B : Type) :=  (A * A * B)%type.
+Definition RG_Edge (A B : Type) :=  (A * A * B)%type.
 
 (* Start defining functionality: *)
 Print RG_empty.
@@ -53,6 +56,34 @@ Print RG_empty.
 Print RG_isEmpty.
 (* Definition RG_isEmpty {A B: Type} (rg : RG A B) : Prop :=
   RG_isEmpty rg. *)
+
+
+
+
+(* Defining equivalences for the sake of proving stuff *)
+
+Definition RG_Adj_equiv {A B : Type} (adj1 adj2 : RG_Adj A B) : Prop :=
+  forall (a : A) (b : B), adj1 b a <-> adj2 b a.
+
+
+Notation "adj1 A== adj2" := (RG_Adj_equiv adj1 adj2) (at level 100, right associativity).
+
+
+Definition RG_Context_equiv {A B : Type} (c1 c2 : RG_Context A B) : Prop :=
+  match c1, c2 with | (fromsC1, nC1, tosC1), (fromsC2, nC2, tosC2) =>
+      nC1 = nC2 /\ RG_Adj_equiv fromsC1 fromsC2 /\ RG_Adj_equiv tosC1 tosC2
+  end
+.
+
+Notation "c1 C== c2" := (RG_Context_equiv c1 c2) (at level 79, right associativity).
+
+Definition RG_Decomp_equiv {A B : Type} (d1 d2 : RG_Decomp A B) : Prop :=
+  match d1, d2 with | ((opt1, context1), rg1), ((opt2, context2), rg2) =>
+    (opt1 <-> opt2) /\ context1 C== context2 /\ (rg1 === rg2)
+  end
+.
+
+Notation "c1 D== c2" := (RG_Decomp_equiv c1 c2) (at level 79, right associativity).
 
 
 
@@ -72,20 +103,23 @@ Defined.
 
 
 (* Checks if the node is in the RG (the Prop return) and returns two sets of alls incoming neighbors and outgoing neighbors *)
-Definition _getFromsAndTos {A B : Type} (node : A) (rg : RG A B) : Prop * Context A B :=
-  (rg.(RG_nodes) node, ((fun l (from : A) => rg.(RG_edges) from node l), node, (fun l (to : A) => rg.(RG_edges) node to l)))
+Definition _getFromsAndTos {A B : Type} (node : A) (rg : RG A B) : Prop * RG_Context A B :=
+  let isValid := rg.(RG_nodes) node in
+  (isValid, ((fun l (from : A) => isValid /\ rg.(RG_edges) from node l),
+              node,
+              (fun l (to : A) => isValid /\ rg.(RG_edges) node to l)))
 .
 
 
-Definition RG_match {A B : Type} (node : A) (rg : RG A B) : (Prop * Context A B) * RG A B :=
+Definition RG_match {A B : Type} (node : A) (rg : RG A B) : RG_Decomp A B :=
   (_getFromsAndTos node rg, _eliminate node rg)
 .
 
 
-Definition _add {A B : Type} (context : Context A B) (rg : RG A B) : RG A B.
+Definition _add {A B : Type} (context : RG_Context A B) (rg : RG A B) : RG A B.
 Proof.
   destruct context as [[froms node] tos].
-  Print Adj.
+  Print RG_Adj.
   refine {|
       RG_nodes := fun (n : A) =>  (exists l, froms l n) \/
                                   (exists l, tos l n) \/
@@ -108,7 +142,7 @@ Definition _insNodes {A B : Type} (nodes : list A) (rg : RG A B) : RG A B :=
 
 
 (* If one of the nodes of the edge does not exist, nothing happens *)
-Definition _insEdge {A B : Type} (edge : Edge A B) (rg : RG A B) : RG A B.
+Definition _insEdge {A B : Type} (edge : RG_Edge A B) (rg : RG A B) : RG A B.
 Proof.
   destruct edge as [[node1 node2] elabel].
     refine {|
@@ -123,10 +157,10 @@ Proof.
 Defined.
 
 
-Definition _insEdges {A B : Type} (edges : list (Edge A B)) (rg : RG A B) : RG A B :=
+Definition _insEdges {A B : Type} (edges : list (RG_Edge A B)) (rg : RG A B) : RG A B :=
   fold_right _insEdge rg edges.
 
-Definition RG_mkGraph {A B : Type} (nodes : list A) (edges : list (Edge A B)) : RG A B :=
+Definition RG_mkGraph {A B : Type} (nodes : list A) (edges : list (RG_Edge A B)) : RG A B :=
   _insEdges edges (_insNodes nodes RG_empty).
  
 
