project/relational_graph_IG_operations_theory.v
@@ -9,26 +9,74 @@ Import ListNotations.
 Require Import MyProject.project.util.util.
 
 (* Require Import MyProject.project.relational_graph.
-Require Import MyProject.project.relational_graph_theory. *)
+ *)
 
 Require Import Coq.Sets.Ensembles.
+Require Import Setoid Morphisms.
+
 
 Require Import MyProject.project.util.NatSet.
 Require Import MyProject.project.relational_graph.
+Require Import MyProject.project.relational_graph_theory.
 Require Import MyProject.project.relational_graph_IG_operations.
 
 
 Open Scope nat_scope.
 
-
 (* Specifies behavior of IH functions on an (edge-label compatible) RG via equational specification *)
+
+
+(* Proving also Adj and Context equivalence relations *)
+
+
+Instance RG_Adj_Equivalence {A B : Type} : Equivalence (@RG_Adj_equiv A B).
+Proof.
+  unfold RG_Adj_equiv. split.
+  - firstorder.
+  - firstorder.
+  - unfold Transitive. firstorder.
+    + apply H0. apply H. assumption.
+    + apply H. apply H0. assumption.
+Qed.
+
+(* Maybe its worth it to make theorem that a conjuction os equivlaence relations is also an equivalence relation *)
+Instance RG_Context_Equivalence {A B : Type} : Equivalence (@RG_Context_equiv A B).
+Proof.
+  unfold RG_Context_equiv. pose proof (@RG_Adj_Equivalence A B). destruct H. split.
+  - unfold Reflexive in *. intros. destruct x as [[froms node] tos]. firstorder.
+  - unfold Symmetric in *. intros.
+    destruct x as [[froms1 node1] tos1]. destruct y as [[froms2 node2] tos2].
+    firstorder.
+  - unfold Transitive in *.
+    destruct x as [[froms1 node1] tos1]. destruct y as [[froms2 node2] tos2]. destruct z as [[froms3 node3] tos3].
+    intros. destruct H as [a1 [b1 c1]]. destruct H0 as [a2 [b2 c2]]. split.
+    + rewrite a1. rewrite a2. reflexivity.
+    + split.
+      -- rewrite b1. rewrite b2. reflexivity.
+      -- rewrite c1. rewrite c2. reflexivity.
+Qed.
+
+
+Instance RG_Decomp_Equivalence {A B : Type} : Equivalence (@RG_Decomp_equiv A B).
+Proof.
+  unfold RG_Decomp_equiv. pose proof (@RG_Context_Equivalence A B). pose proof (@RG_Equivalence A B). destruct H. destruct H0. split.
+  - unfold Reflexive in *. intros. destruct x as [[opt context] rg]. firstorder.
+  - unfold Symmetric in *. intros.
+    destruct x as [[opt1 context1] rg1]. destruct y as [[opt2 context2] rg2].
+    firstorder.
+  - unfold Transitive in *.
+    destruct x as [[opt1 context1] rg1]. destruct y as [[opt2 context2] rg2]. destruct z as [[opt3 context3] rg3].
+    firstorder.
+    + apply H3. apply H7. assumption.
+    + apply H7. apply H3. assumption.
+Qed.
 
 
 (* 5 statements on inserting (helpers for mkGraph): update, insEdge, insEdges, insNode, insNodes *)
 
 
 
-Lemma RG_insEdge_does_not_add_node : forall (A B : Type) (edge : (Edge A B)) (rg : RG A B),
+Lemma RG_insEdge_does_not_add_node : forall (A B : Type) (edge : (RG_Edge A B)) (rg : RG A B),
   RG_labNodes (_insEdge edge rg) S== RG_labNodes rg.
 Proof.
   intros.
@@ -37,7 +85,7 @@ Qed.
 
 
 
-Lemma RG_insEdges_does_not_add_nodes : forall (A B : Type) (edges : list (Edge A B)) (rg : RG A B),
+Lemma RG_insEdges_does_not_add_nodes : forall (A B : Type) (edges : list (RG_Edge A B)) (rg : RG A B),
   RG_labNodes (_insEdges edges rg) S== RG_labNodes rg.
 Proof.
   intros.
@@ -71,7 +119,7 @@ Qed.
 
 
 
-Lemma RG_insEdge_on_empty_is_empty : forall (A B : Type) (edge : (Edge A B)),
+Lemma RG_insEdge_on_empty_is_empty : forall (A B : Type) (edge : (RG_Edge A B)),
   _insEdge edge RG_empty === RG_empty.
 Proof.
   intros. unfold RG_equiv. destruct edge as [[from to] lab]. split.
@@ -81,7 +129,7 @@ Qed.
 
 
 
-Lemma RG_insEdges_on_empty_is_empty : forall (A B : Type) (edges : list (Edge A B)),
+Lemma RG_insEdges_on_empty_is_empty : forall (A B : Type) (edges : list (RG_Edge A B)),
   _insEdges edges RG_empty === RG_empty.
 Proof.
   intros. pose proof RG_insEdge_on_empty_is_empty. induction edges.
@@ -93,7 +141,7 @@ Qed.
 
 
 (* "big" statement: *)
-Theorem RG_mkGraph_any_ins_all_nodes : forall (A B : Type) (nodes : list A) (edges : list (Edge A B)),
+Theorem RG_mkGraph_any_ins_all_nodes : forall (A B : Type) (nodes : list A) (edges : list (RG_Edge A B)),
   RG_labNodes (RG_mkGraph nodes edges) S== cListToEnsemble nodes.
 Proof.
   intros.
@@ -119,7 +167,7 @@ Proof.
   firstorder.
 Qed.
 
-(* Lemma RG_ins_only_edge_isEmpty : forall (A B : Type) (edge : (Edge A B)),
+(* Lemma RG_ins_only_edge_isEmpty : forall (A B : Type) (edge : (RG_Edge A B)),
   _insEdge edge RG_empty === RG_empty.
 Proof.
   intros. unfold RG_equiv. destruct edge as [[from to] lab]. split.
@@ -128,14 +176,14 @@ Proof.
 Qed. *)
 
 
-Lemma RG_ins_only_edge_isEmpty : forall (A B : Type) (edge : Edge A B) (rg : RG A B),
+Lemma RG_ins_only_edge_isEmpty : forall (A B : Type) (edge : RG_Edge A B) (rg : RG A B),
   RG_isEmpty rg <-> RG_isEmpty (_insEdge edge rg).
 Proof.
   intros. destruct edge as [[from to] lab]. firstorder.
 Qed.
 
 
-Lemma RG_ins_only_edges_isEmpty : forall (A B : Type) (edges : list (Edge A B)) (rg : RG A B),
+Lemma RG_ins_only_edges_isEmpty : forall (A B : Type) (edges : list (RG_Edge A B)) (rg : RG A B),
   RG_isEmpty rg <-> RG_isEmpty (_insEdges edges rg).
 Proof.
   intros. induction edges; simpl in *.
@@ -167,14 +215,16 @@ Qed.
 
 
 Theorem RG_match_empty_is_nothing : forall (A B : Type) (node : A),
-  RG_match node (@RG_empty A B) = ((False, (fun x y => False, node, fun x y => False)), RG_empty).
+  RG_match node (@RG_empty A B) D== ((False, (fun x y => False, node, fun x y => False)), RG_empty).
 Proof.
-Admitted.
+  firstorder.
+Qed.
 
 
 
 
-(* Theorem RG_spec4 : forall (A B : Type) (node : A) (nodes : list A) (edges : list (Edge A B)), 
+
+(* Theorem RG_spec4 : forall (A B : Type) (node : A) (nodes : list A) (edges : list (RG_Edge A B)), 
   List.In node nodes -> exists froms tos, RG_match node (RG_mkGraph nodes edges) =
   ((True, (froms, tos)), RG_mkGraph (filter (fun n => negb (node =? n)) nodes) (filter (fun '(from, to) => negb ((from =? node) || (to =? node))) edges)).
 (* This is not even a complete specification and it looks like a hard one to prove... *)
@@ -182,7 +232,20 @@ Proof.
 Admitted. *)
 
 
-Theorem RG_spec5 : forall (A B : Type) (node : A) (nodes : list A) (edges : list (Edge A B)), 
-  not (List.In node nodes) -> RG_match node (RG_mkGraph nodes edges) = ((False, (fun x y => False, node, fun x y => False)), RG_mkGraph nodes edges).
+
+
+
+Theorem RG_spec5 : forall (A B : Type) (node : A) (nodes : list A) (edges : list (RG_Edge A B)), 
+  not (List.In node nodes) ->
+    RG_match node (RG_mkGraph nodes edges) = ((False, (fun x y => False, node, fun x y => False)), RG_mkGraph nodes edges).
 Proof.
+  intros.
+  unfold not in H. unfold RG_match. f_equal.
+  - unfold _getFromsAndTos. f_equal.
+    +  admit.
+    + f_equal.
+      -- f_equal.
+        ++ admit.
+      -- admit.
+  - admit.
 Admitted.
